src/lib/FreeC/Backend/Coq/Converter/Expr.hs
@@ -76,15 +76,14 @@ convertLiftedExpr (LIR.Share _ arg argType) = do
   argType' <- mapM convertLiftedType argType
   return
     $ genericApply' (Coq.Qualid Coq.Base.share)
-    [genericApply Coq.Base.strategyArg [Coq.Underscore] [] []] []
-    (maybeToList argType') [Coq.Base.implicitArg] [arg']
+    [Coq.Qualid Coq.Base.strategyArg] [] (maybeToList argType')
+    [Coq.Base.implicitArg] [arg']
 convertLiftedExpr (LIR.Call _ arg argType) = do
   arg' <- convertLiftedExpr arg
   argType' <- mapM convertLiftedType argType
   return
     $ genericApply' (Coq.Qualid Coq.Base.call)
-    [genericApply Coq.Base.strategyArg [Coq.Underscore] [] []] []
-    (maybeToList argType') [] [arg']
+    [Coq.Qualid Coq.Base.strategyArg] [] (maybeToList argType') [] [arg']
 
 -- | Converts a Haskell expression to Coq.
 convertExpr :: IR.Expr -> Converter Coq.Term
