base/coq/Free/Class/ShareableArgs.v
@@ -1,13 +1,18 @@
+From Base Require Import Free.Class.Strategy.
 From Base Require Import Free.Monad.
 
-Class ShareableArgs (Shape : Type) (Pos : Shape -> Type)
-                    (A : Type) :=
-  {
-    shareArgs : A -> Free Shape Pos A
-  }.
+Class ShareableArgs (Shape : Type) (Pos : Shape -> Type) (A : Type) :=
+  { shareArgs : Strategy Shape Pos -> A -> Free Shape Pos A }.
 
 (* ShareableArgs instance for functions.
    Effects inside of functions are not shared. *)
 Instance ShareableArgsFunc (Shape : Type) (Pos : Shape -> Type) (A B : Type)
  : ShareableArgs Shape Pos (A -> B) :=
-  { shareArgs := pure }.
+  { shareArgs _ := pure }.
+
+(* Share operator with deep sharing. *)
+Definition share (Shape : Type) (Pos : Shape -> Type)
+                 (S : Strategy Shape Pos)
+                 {A : Type} `{ShareableArgs Shape Pos A}
+  : Free Shape Pos A -> Free Shape Pos (Free Shape Pos A)
+ := shareWith Shape Pos S shareArgs.
