example/Base/SharingProofs.v
@@ -7,9 +7,8 @@ Theorem cbn_no_sharing : forall (A : Type)
                                 (B : Type)
                                 (Shape : Type)
                                 (Pos : Shape -> Type)
-                                `{I : Injectable Share.Shape Share.Pos Shape Pos}
                                 `{SA : ShareableArgs Shape Pos A}
                                 (fx : Free Shape Pos A)
                                 (f : Free Shape Pos A -> Free Shape Pos B),
-  @share Shape Pos (Cbn Shape Pos) A SA fx >>= f = f fx.
+  @share Shape Pos Cbn A SA fx >>= f = f fx.
 Proof. constructor. Qed.
