example/CaseStudyHuttonsRazor/RazorProofsPureCodes.v
@@ -48,7 +48,6 @@ Section Proofs_PureCodes.
 
   Variable Shape   : Type.
   Variable Pos     : Shape -> Type.
-  Context `{Injectable Share.Shape Share.Pos Shape Pos}.
   Variable Partial : Partial Shape Pos.
 
   (* If the code is pure and the first operation is pure if there is any, the
