example/Proofs/ConsUnconsProofs.v
@@ -6,18 +6,14 @@ Require Import Coq.Logic.FunctionalExtensionality.
 (* The first QuickCheck property holds for any [Partial] instance. Therefore
    its proof differs only in that way from proofs about functions that do not
    return an error, that an [Partial] instance for [Shape] and [Pos] is given. *)
-Lemma cons_unconsE : quickCheck (fun Shape Pos I => @prop_cons_unconsE Shape Pos I Cbn).
+Lemma cons_unconsE : quickCheck (fun Shape Pos => @prop_cons_unconsE Shape Pos Cbn).
 Proof.
-  intros Shape Pos I Partial A SA NF fx fxs.
+  intros Shape Pos Partial A SA NF fx fxs.
   reflexivity.
 Qed.
 
 (* The second QuickCheck property holds provably for the [Maybe] instance of [Partial]. *)
-Lemma unconsE_fst_Maybe : quickCheck (@prop_unconsE_fst 
-    (Comb.Shape Share.Shape Maybe.Shape)
-    (Comb.Pos Share.Pos Maybe.Pos)
-    _ Cbn
-    (Maybe.Partial _ _)).
+Lemma unconsE_fst_Maybe : quickCheck (@prop_unconsE_fst Maybe.Shape Maybe.Pos Cbn (Maybe.Partial _ _)).
 Proof.
   intros A SA NF fxs.
   simpl.
@@ -26,21 +22,13 @@ Proof.
     + simpl. unfold Nothing. f_equal. extensionality p. destruct p.
     + reflexivity.
   - simpl. f_equal. extensionality p. destruct s.
-    (* Because the Share effect is required in the effect stack even though
-       call-by-name evaluation is used, an impure value could theoretically consist
-       of sharing syntax, even though sharing syntax is never used in this setting. *)
-    + admit.
-    (* The Maybe effect does not have any positions. *)
-    + destruct p. Admitted.
+    + destruct p.
+Qed.
 
 (* But the second QuickCheck property doesn't hold for the [Error] instance of
    [Partial] as [unconsE] and [head] have different error messages on an empty
    list. *)
-Lemma unconsE_fst_Error : not (quickCheck (@prop_unconsE_fst 
-  (Comb.Shape Share.Shape (Error.Shape string))
-  (Comb.Pos Share.Pos Error.Pos) 
-   _ Cbn
-  (Error.Partial _ _))).
+Lemma unconsE_fst_Error : not (quickCheck (@prop_unconsE_fst (Error.Shape string) Error.Pos Cbn (Error.Partial _ _))).
 Proof.
   intro H.
   specialize (H bool _ _ (Nil _ _)).
