example/Proofs/ReverseInvolutiveProofs.v
@@ -9,9 +9,7 @@ Require Import Coq.Logic.FunctionalExtensionality.
 (* In order to prove that [reverse] is not involutive in a partial setting
    consider the counterexample defined in Haskell and the [Maybe] monad. *)
 Example partial_reverse_non_involutive:
-  ~quickCheck (@prop_reverse_involutive 
-  (Comb.Shape Share.Shape Maybe.Shape)
-  (Comb.Pos Share.Pos Maybe.Pos) _ Cbn).
+  ~quickCheck (@prop_reverse_involutive Maybe.Shape  Maybe.Pos Cbn).
 Proof.
   simpl. intros H.
   discriminate 
@@ -23,9 +21,7 @@ Qed.
    However, we have to prove the following lemma first. *)
 
 Lemma total_reverse_append_singleton: 
-  quickCheck (@prop_reverse_append_singleton 
-    (Comb.Shape Share.Shape Identity.Shape) 
-    (Comb.Pos Share.Pos Identity.Pos) _ Cbn).
+  quickCheck (@prop_reverse_append_singleton Identity.Shape Identity.Pos Cbn).
 Proof.
   intros a SA NF fxs fx.
   simpl. induction fxs using FreeList_ind 
@@ -34,16 +30,13 @@ Proof.
   - (* fxs = pure (cons fxs1 fxs2) *)
     simpl. destruct fxs2 as [xs2 | s pf].
     + (* fxs2 = pure xs2 *)    simpl in *. unfold reverse in IHfxs1. rewrite IHfxs1. reflexivity.
-    + (* fxs2 = impure s pf *) destruct s. 
-      (* We need to consider sharing syntax here. *) admit. admit.
+    + (* fxs2 = impure s pf *) destruct s.
   - (* fxs = pure xs *)    apply IHfxs.
   - (* fxs = impure _ _ *) destruct s.
-Admitted.
+Qed.
 
 Theorem total_reverse_involutive:
-  quickCheck (@prop_reverse_involutive
-    (Comb.Shape Share.Shape Identity.Shape) 
-    (Comb.Pos Share.Pos Identity.Pos) _ Cbn).
+  quickCheck (@prop_reverse_involutive Identity.Shape Identity.Pos Cbn).
 Proof.
   intros a SA NF fxs.
   simpl. induction fxs using FreeList_ind 
@@ -56,9 +49,8 @@ Proof.
     do 2 apply f_equal. destruct fxs2 as [xs2 | s pf].
     + (* fxs2 = pure xs2 *)    simpl. apply IHfxs1.
     + (* fxs2 = impure s pf *) destruct s.
-      (* We need to consider sharing syntax here. *) admit. admit.
   - (* fxs = pure xs *)
     simpl. apply IHfxs.
   - (* fxs = impure s pf *)
     destruct s.
-Admitted.
+Qed.
