example/Proofs/TracingProofs.v
@@ -3,6 +3,6 @@ From Generated Require Import Proofs.Tracing.
 
 Theorem trace_is_shared : quickCheck prop_trace_is_shared.
 Proof.
-  intros Shape Pos I S T. simpl.
+  intros Shape Pos S T. simpl.
   (* TODO Complete prove once [quickCheck] is parameterized over handler. *)
 Admitted.
