example/Queue/Queue.v
@@ -70,9 +70,9 @@ Proof.
   - (* fb1 = impure _ _, fb2 = impure _ _ *) contradiction Hpure.
 Qed.
 
-Lemma null_rev : quickCheck (fun Shape Pos I => @prop_null_rev Shape Pos I Cbn).
+Lemma null_rev : quickCheck (fun Shape Pos => @prop_null_rev Shape Pos Cbn).
 Proof.
-  intros Shape Pos I a SA fxs Hnull.
+  intros Shape Pos a SA fxs Hnull.
   destruct fxs as [ xs |  ].
   - (* fxs = pure xs *)
     destruct xs.
@@ -82,9 +82,9 @@ Proof.
     contradiction Hnull.
 Qed.
 
-Lemma append_nil : quickCheck (fun Shape Pos I => @prop_append_nil Shape Pos I Cbn).
+Lemma append_nil : quickCheck (fun Shape Pos => @prop_append_nil Shape Pos Cbn).
 Proof.
-  intros Shape Pos I a SA NF fxs.
+  intros Shape Pos a SA NF fxs.
   induction fxs using FreeList_ind with (P := fun xs => append1 Shape Pos a (pure nil) Cbn xs = pure xs); simpl.
   - reflexivity.
   - simpl; repeat apply f_equal. apply IHfxs1.
@@ -95,7 +95,6 @@ Qed.
 Lemma append1_assoc :
   forall (Shape : Type)
          (Pos : Shape -> Type)
-         `{Injectable Share.Shape Share.Pos Shape Pos}
          {a : Type}
          `{ShareableArgs Shape Pos a}
          (xs : List Shape Pos a)
@@ -103,7 +102,7 @@ Lemma append1_assoc :
       append1 Shape Pos a (append Shape Pos Cbn fys fzs) Cbn xs
       = append Shape Pos Cbn (append1 Shape Pos a fys Cbn xs) fzs.
 Proof.
-  intros Shape Pos I a SA xs fys fzs.
+  intros Shape Pos a SA xs fys fzs.
   induction xs.
   - reflexivity.
   - induction fxs.
@@ -113,9 +112,9 @@ Proof.
       simplify H as IH. apply IH.
 Qed.
 
-Lemma append_assoc : quickCheck (fun Shape Pos I => @prop_append_assoc Shape Pos I Cbn).
+Lemma append_assoc : quickCheck (fun Shape Pos => @prop_append_assoc Shape Pos Cbn).
 Proof.
-  intros Shape Pos I a SA NF fxs fys fzs.
+  intros Shape Pos a SA NF fxs fys fzs.
   induction fxs as [ | s pf IH ].
   - simpl. apply append1_assoc.
   - (*Inductive case: [fxs = impure s pf] with induction hypothesis [IH] *)
@@ -133,13 +132,12 @@ Definition singleton (Shape : Type)
 (* QuickCheck properties *)
 Theorem prop_isEmpty_theorem : forall (Shape : Type)
   (Pos : Shape -> Type)
-  `{I : Injectable Share.Shape Share.Pos Shape Pos}
   {a : Type} `{SA : ShareableArgs Shape Pos a} `{NF : Normalform Shape Pos a}
   (total_a : Free Shape Pos a -> Prop)
   (qi : Free Shape Pos (QueueI Shape Pos a)),
-  total_queue Shape Pos total_a qi -> quickCheck (@prop_isEmpty Shape Pos I Cbn a SA NF qi).
+  total_queue Shape Pos total_a qi -> quickCheck (@prop_isEmpty Shape Pos Cbn a SA NF qi).
 Proof.
-  intros Shape Pos I a SA NF total_a fqi Htotal Hinv.
+  intros Shape Pos a SA NF total_a fqi Htotal Hinv.
   destruct fqi as [qi | ].
   - (* fqi = pure qi *)
     destruct qi as [fxs fys]. (* qi = (fxs, fys) *)
@@ -150,7 +148,7 @@ Proof.
         simpl in *. apply (is_pure_true_or Shape Pos) in Hinv.
         destruct Hinv as [Hnull | Hcontra].
         -- (* null Shape Pos fys *)
-           apply (null_rev Shape Pos I a SA) in Hnull.
+           apply (null_rev Shape Pos a SA) in Hnull.
            symmetry. unfold isEmpty. apply pure_bool_toProperty in Hnull. apply Hnull.
         -- (* False_ Shape Pos *)
            discriminate Hcontra.
@@ -163,9 +161,9 @@ Proof.
 Qed.
 
 (* In fact we do not need the totality constraint in this case. *)
-Theorem prop_isEmpty_theorem' : quickCheck (fun Shape Pos I => @prop_isEmpty Shape Pos I Cbn).
+Theorem prop_isEmpty_theorem' : quickCheck (fun Shape Pos => @prop_isEmpty Shape Pos Cbn).
 Proof.
-  intros Shape Pos I a SA NF fqi Hinv.
+  intros Shape Pos a SA NF fqi Hinv.
   destruct fqi as [qi | ].
   - (* fqi = pure qi *)
     destruct qi as [fxs fys]. (* qi = (fxs, fys) *)
@@ -176,7 +174,7 @@ Proof.
         simpl in *. apply is_pure_true_or in Hinv.
         destruct Hinv as [Hnull | Hcontra].
         -- (* null Shape Pos fys *)
-           apply (null_rev Shape Pos I a SA) in Hnull.
+           apply (null_rev Shape Pos a SA) in Hnull.
            symmetry. unfold isEmpty. apply pure_bool_toProperty in Hnull. apply Hnull.
         -- (* False_ Shape Pos *)
            discriminate Hcontra.
@@ -187,10 +185,10 @@ Proof.
       destruct Hinv as [Hnull | Hcontra].
       -- (* null Shape Pos fys *)
          apply f_equal, functional_extensionality. intros x.
-         apply (null_rev Shape Pos I a SA) in Hnull.
+         apply (null_rev Shape Pos a SA) in Hnull.
          destruct (reverse Shape Pos Cbn fys) as [[| y ys'] |].
          ++ (* reverse Shape Pos fys = Nil Shape Pos *)
-            specialize (append_nil Shape Pos I a SA NF) as appNil.
+            specialize (append_nil Shape Pos a SA NF) as appNil.
             simpl in appNil. unfold isEmpty. rewrite appNil. reflexivity.
          ++ (* reverse Shape Pos fys = Cons Shape Pos y ys' *)
             simpl in Hnull. discriminate Hnull.
@@ -203,22 +201,22 @@ Proof.
 Qed.
 
 (* In order to prove [prop_add] no totality constraint is necessary. *)
-Theorem prop_add_theorem : quickCheck (fun Shape Pos I => @prop_add Shape Pos I Cbn).
+Theorem prop_add_theorem : quickCheck (fun Shape Pos => @prop_add Shape Pos Cbn).
 Proof.
-  intros Shape Pos I a SA NF fx fqi.
+  intros Shape Pos a SA NF fx fqi.
   induction fqi as [ [f1 f2] | eq ]; simpl.
   - destruct f1 as [l | s pf]; simpl.
     + destruct l as [ | fy fys]; simpl.
-      * specialize (append_nil Shape Pos I a SA NF) as appNil. simpl in appNil.
+      * specialize (append_nil Shape Pos a SA NF) as appNil. simpl in appNil.
         rewrite appNil. reflexivity.
-      * apply (append_assoc Shape Pos I _ SA NF (pure (cons fy fys))
+      * apply (append_assoc Shape Pos _ SA NF (pure (cons fy fys))
           (reverse Shape Pos Cbn f2) (singleton Shape Pos fx)).
     + unfold add. simpl. repeat apply f_equal. extensionality p.
       induction (pf p) as [fys |]; simpl.
       * destruct fys; simpl.
-        -- specialize (append_nil Shape Pos I a SA NF) as appNil. simpl in appNil. rewrite appNil.
+        -- specialize (append_nil Shape Pos a SA NF) as appNil. simpl in appNil. rewrite appNil.
            reflexivity.
-        -- do 2 apply f_equal. apply (append_assoc Shape Pos I _ SA NF f0 (reverse Shape Pos Cbn f2) (singleton Shape Pos fx)).
+        -- do 2 apply f_equal. apply (append_assoc Shape Pos _ SA NF f0 (reverse Shape Pos Cbn f2) (singleton Shape Pos fx)).
       * repeat apply f_equal.
         extensionality p1.
         apply H.
@@ -228,10 +226,10 @@ Proof.
 Qed.
 
 (* We have to add a totality constraint to [prop_front]. *)
-Theorem prop_front_theorem : forall Shape Pos I P a NF SA total_a qi,
-  total_queue Shape Pos total_a qi -> quickCheck (@prop_front Shape Pos I Cbn P a SA NF qi).
+Theorem prop_front_theorem : forall Shape Pos P a NF SA total_a qi,
+  total_queue Shape Pos total_a qi -> quickCheck (@prop_front Shape Pos Cbn P a SA NF qi).
 Proof.
-  intros Shape Pos I P a total_a SA NF fqi Htotal HinvNempty.
+  intros Shape Pos P a total_a SA NF fqi Htotal HinvNempty.
   apply is_pure_true_and in HinvNempty.
   destruct HinvNempty as [Hinv Hnempty].
   destruct Htotal as [ff fb Htotal1 Htotal2]. (* fqi = pure (ff, fb) *)
@@ -245,16 +243,16 @@ Qed.
 
 (* Since the compiler is now adding vanishing type arguments automatically,
    the [prop_inv_empty] can be proven without a problem. *)
-Theorem prop_inv_empty_theorem : quickCheck (fun Shape Pos I => @prop_inv_empty Shape Pos I Cbn).
+Theorem prop_inv_empty_theorem : quickCheck (fun Shape Pos => @prop_inv_empty Shape Pos Cbn).
 Proof.
   intros Shape Pos I t0. simpl. reflexivity.
 Qed.
 
 (* Proving [prop_inv_add] requires a totality constraint.
    Otherwise we get stuck in the case admitted below. *)
-Theorem prop_inv_add_theorem : quickCheck (fun Shape Pos I => @prop_inv_add Shape Pos I Cbn).
+Theorem prop_inv_add_theorem : quickCheck (fun Shape Pos => @prop_inv_add Shape Pos Cbn).
 Proof.
-  intros Shape Pos I a SA fx fq H. destruct fq as [[ff fb] |].
+  intros Shape Pos a SA fx fq H. destruct fq as [[ff fb] |].
   - (* fq = Pair_ Shape Pos ff fb *)
     destruct ff as [f |]; destruct fb as [b |].
     + (* ff = pure f; fb = pure b *)
@@ -275,10 +273,10 @@ Abort.
 
 (* To add the totality constraint we have to introduce all arguments of [prop_inv_add]
    first. However, we do not have to repeat the type annotations here. *)
-Theorem prop_inv_add_theorem : forall Shape Pos I a SA total_a x q,
-  total_queue Shape Pos total_a q -> quickCheck (@prop_inv_add Shape Pos I Cbn a SA x q).
+Theorem prop_inv_add_theorem : forall Shape Pos a SA total_a x q,
+  total_queue Shape Pos total_a q -> quickCheck (@prop_inv_add Shape Pos Cbn a SA x q).
 Proof.
-  intros Shape Pos I a SA total_a fx fq Htotal H.
+  intros Shape Pos a SA total_a fx fq Htotal H.
   destruct Htotal as [ff fb HtotalF HtotalB]. (* fq = Pair_ ff fb *)
   destruct HtotalF; reflexivity.
 Qed.
